---
UID: 20240713134532 
aliases: 
tags: 
source: 
cssclass: 
created: 2024-07-13
---

## ✍内容
Euler’s product formula
> [!thm]
> For every $\displaystyle s>1$, we have
> $$
\zeta(s)=\prod_{p} \frac{1}{1-1/p^{s}}
$$

where the product is taken over all primes.[[Stein-I-Fourier Analysis.pdf#page=266&rect=31,370,336,444|Stein-I-Fourier Analysis, p.249]]

> [!def]
> Dirichlet characters modulo $\displaystyle q$
> [[Stein-I-Fourier Analysis.pdf#page=271|Stein-I-Fourier Analysis, p.254]]


> [!def]
> Charaters:
> Let $\displaystyle G$ be a finite abelian group (with multiplication), and $\displaystyle S^{1}$ be the unit circle in the complex plane. A character on $\displaystyle G$ is a complex-valued function $\displaystyle e:G\to S^{1}$ which satisfies the following condition:
> $$
e(a\cdot b)=e(a)e(b)\ \ \ \ \text{for all }a,b\in G
$$

And we denote by $\displaystyle \hat{G}$ the set of all characters of $\displaystyle G$, and observe that this set inherits the structure of an abelian group.
> [!NOTE]
> 这里 $\displaystyle G$ 与 $\displaystyle \text{Hom}(G,S^{1})$ 是范畴等价的，所以 $\displaystyle G$ 中的一个对象对应 $\displaystyle \text{Hom}(G,S^{1})$ 中的一个对象. 

Take an abelian group $\displaystyle G$ to be $\displaystyle \mathbb{Z}_{q}^{\times}$, and $\displaystyle \lvert G \rvert=\varphi(q)$.
Consider the characteristic function of $\displaystyle l$
$$
\delta_{l}(n)=\left\{\begin{array}{l}
1 & \text{if } n\equiv l \text{ mod }q \\
0 & \text{otherwise}
\end{array}\right.
$$
We can expand this function in a Fourier series as follows:
$$
\delta_{l}(n)=\sum_{e\in \hat{G}}\hat{\delta}_{l}(e)e(n)
$$
Where
$$
\hat{\delta}_{l}(e)= \frac{1}{\lvert G \rvert }\sum_{m\in G}\delta_{l}(m) \overline{e(m)}= \frac{1}{\lvert G \rvert }\overline{e(l)}
$$
Hence
$$
\delta _{l}(n)=\underset{ 也就是把每个e(l)都拿过来作用一下 }{ \frac{1}{\lvert G \rvert }\sum_{e\in \hat{G}} \overline{e(l)}e(n) }
$$
We can extend the function $\displaystyle \delta_{l}$ to all of $\displaystyle \mathbb{Z}$ by setting $\displaystyle \delta_{l}(m)=0$ whenever $\displaystyle m$ and $\displaystyle q$ are not relatively prime. Similarly, the extensions of the characters $\displaystyle e\in \hat{G}$ to all of $\displaystyle \mathbb{Z}$ which are given by the recipe
$$
\chi(m)=\left\{\begin{array}{l}
e(m) & \text{if }m \text{ and }q \text{ are relatively prime} \\
0 & \text{otherwise} 
\end{array}\right.

$$
这个 $\displaystyle \chi(m)$ 就叫做 Dirichlet character modulo $\displaystyle q$. 并且补充定义 $\displaystyle \hat{G}$ 中的 trivial character $\displaystyle \chi_{0}$, 即上式的 $\displaystyle e (m)\equiv 1$.

> [!lem] 
> 由上面的形式，将 Dirichlet character 带入可以知道：
> $$
\delta_{l}(m)=\frac{1}{\varphi(q)}\sum_{\chi} \overline{\chi(l)}\chi (m) 
$$

这里的求和表示对所有的 Dirichlet characters. 
Application of the lemma follows:
$$
\begin{align}
\sum_{p\equiv l} \frac{1}{p^{s}} & =\sum_{p} \frac{\delta_{l}(p)}{p^{s}} \\
 & =\frac{1}{\varphi(q)}\sum_{\chi}\overline{\chi(l)}\sum_{p} \frac{\chi(p)}{p^{s}} \\
 & =\frac{1}{\varphi(q)}\sum_{p} \frac{\chi_{0}(p)}{p^{s}}+ \frac{1}{\varphi(q)}\sum_{\chi\neq \chi_{0}} \overline{\chi(l)}\sum_{p} \frac{\chi(p)}{p^{s}} \\
 & =\frac{1}{\varphi(q)}\underbrace{ \sum_{p\text{ not dividing }q} \frac{1}{p^{s}}}_{ 发散 } + \frac{1}{\varphi(q)}\sum_{\chi\neq \chi_{0}}\overline{\chi(l)}\underbrace{ \sum_{p} \frac{\chi(p)}{p^{s}} }_{ 有界(由接下来的引理) }
\end{align}
$$
> [!lem]
> If $\displaystyle \chi$ is a nontrivial Dirichlet character, then the sum is bounded as $\displaystyle s\to 1^{+}$
> $$
\sum _{p} \frac{\chi(p)}{p^{s}}
$$

The proof requires higher technique, $\displaystyle L-$ functions, to be introduced as follow.

---
We've proved that
$$
\zeta(s)=\sum_{n=1}^{\infty} \frac{1}{n^{s}}=\prod_{p} \frac{1}{1-p^{-s}}
$$
Dirichlet observed an analogue of this formula for the so-called $\displaystyle L-$ functions defined for $\displaystyle s>1$ by
$$
L(s,\chi)=\sum_{n=1}^{\infty}  \frac{\chi(n)}{n^{s}}
$$
where $\displaystyle \chi$ is a Dirichlet character.
> [!thm]
> If $\displaystyle s>1$, then
> $$
\sum_{n=1}^{\infty}  \frac{\chi(n)}{n^{s}}=\prod_{p} \frac{1}{1-\chi(p)p^{-s}}
$$


> [!NOTE]
> The logarithm of a product of complex numbers is not the sum of the logarithms.
> $$
\log(c_{1}c_{2}\dots c_{n})\neq \log c_{1}+\log c_{2}+\dots+\log c_{n}\ \ \ \ \text{where }c_{i}\in \mathbb{C}
 $$

$$
e^{A}=e^{B}(A,B\in \mathbb{C})\implies A=B+2\pi i \cdot M\ \ \ \ \text{where }M\in \mathbb{Z}
$$
Then
$$
\log(c_{1}c_{2}\dots c_{n})=\log c_{1}+\log c_{2}+\dots+\log c_{n}+2\pi i\cdot M\ \ \ \ \text{where }M\in \mathbb{Z}
$$
We will focus on three points:
1. Complex logarithm and infinite products.
2. Study of $\displaystyle L(s,\chi)$.
3. Proof of $\displaystyle L(1,\chi)\neq0$ if $\displaystyle \chi$ is non-trivial.

---
### Logarithm
First to define two logarithms: [[Stein-I-Fourier Analysis.pdf#page=275|Stein-I-Fourier Analysis, p.258]]
For the first logarithm, we define:
$$
\log_{1}\left( \frac{1}{1-z} \right)=\sum_{k=1}^{\infty} \frac{z^{k}}{k}\text{   for }\lvert z \rvert <1.

$$
It satisfies the following property:
1. If $\displaystyle \lvert z \rvert<1$, then 
$$
e^{\log_{1}(1/1-z)}=\frac{1}{1-z}
$$
2. If $\displaystyle \lvert z \rvert<1$, then
$$
\log_{1}\left( \frac{1}{1-z} \right)=z+\underbrace{ E_{1}(z) }_{ \lvert E_{1} (z)\rvert<\lvert z \rvert ^{2}  \text{if }\lvert z \rvert <1/2}
$$
3. If $\displaystyle \lvert z \rvert<1/2$, then
$$
\left\lvert  \log_{1}\left( \frac{1}{1-z} \right)  \right\rvert \leq 2\lvert z \rvert
$$
> [!NOTE]
> If $\displaystyle \sum \lvert a_{n} \rvert$ converges, and $\displaystyle a_{n}\neq1$ for all $\displaystyle n$, then
> $$
\prod_{n=1}^{\infty} \left( \frac{1}{1-a_{n}} \right)
$$

converges. Moreover, this product is non-zero.
The above proposition is a direct consequence of the property (3) of $\displaystyle \log_{1}$.
> [!NOTE]
> Motivation of the complete proof. [[Stein-I-Fourier Analysis.pdf#page=277|Stein-I-Fourier Analysis, p.260]]

### L-functions
![[Stein-I-Fourier Analysis.pdf#page=278&rect=33,239,375,397|Stein-I-Fourier Analysis, p.261]]

Property of $\displaystyle L(s,\chi)$: [[Stein-I-Fourier Analysis.pdf#page=278&rect=35,28,386,196|Stein-I-Fourier Analysis, p.261]]
> [!def]
> If $\displaystyle \chi$ is a non-trivial Dirichlet character and $\displaystyle s>1$ we define
> $$
\log_{2}L(s,\chi)=-\int_{s}^{\infty}  \frac{L'(t,\chi)}{L(t,\chi)} \, dt
$$

We know that $\displaystyle L(t,\chi)\neq0$ for every $\displaystyle t>1$ since it is given by a product, and the integral is convergent because
$$
\frac{L'(t,\chi)}{L(t,\chi)}=O(e^{-ct})
$$
Since $\displaystyle L'(t,\chi)=O(e^{-ct}),L(t,\chi)=1+O(e^{-ct})$ as $\displaystyle t\to \infty$.
> [!NOTE]
> If $\displaystyle s>1$, then
> $$
e^{\log_{2}L(s,\chi)}=L(s,\chi)
$$

Moreover
$$
\log_{2}L(s,\chi)=\sum_{p}\log_{1}\left( \frac{1}{1-\chi(p)/p^{s}} \right)
$$
Prove by differentiating $\displaystyle e^{-\log_{2}L(s,\chi)}L(s,\chi)$ with respect to $\displaystyle s$.
### Non-vanishing of the L-function
> [!thm]
> If $\displaystyle \chi\neq \chi_{0}$, then $\displaystyle L (1,\chi)\neq 0.$

The proof may involve algebraic number theory (among them Dirichlet's original argument), or complex analysis. But here we opt for a more elementary argument.
- Case 1: Complex Dirichlet characters

The proof is by contradiction.
> [!lem]
> If $\displaystyle s>1$, then
> $$
\prod_{\chi}L(s,\chi)\geq 1
$$

For $\displaystyle s>1$, we have
$$
L(s,\chi)=\exp \left( \sum_{p}\log_{1}\left( \frac{1}{1-\chi(p)p^{-s}} \right) \right)
$$
Hence,
$$
\begin{align}
\prod_{\chi}L(s,\chi) & =\exp\left( \sum_{\chi}\sum_{p}\log_{1}\left( \frac{1}{1-\chi(p)p^{-s}} \right) \right) \\
 & \overset{ 由定义 }{ = }\exp\left( \sum_{\chi}\sum_{p}\sum_{k=1}^{\infty}  \frac{1}{k} \frac{\chi(p^{k})}{p^{ks}} \right) \\
 & \overset{换序}{ = }\exp\left( \sum_{p}\sum_{k=1}^{\infty} \sum_{\chi} \frac{1}{k} \frac{\chi(p^{k})}{p^{ks}} \right)
\end{align}
$$
由 $\displaystyle \delta_{l}(m)=\frac{1}{\varphi (q)} \sum_{\chi}\overline{\chi(l)}\chi(m)$ 可知，令 $\displaystyle l=1,m=p^{k}$，于是
$$
\sum_{\chi}\chi(p^{k})=\varphi(q)\delta_{1}(p^{k})
$$
于是
$$
\prod_{\chi}L(s,\chi)=\exp\left( \varphi(q)\sum_{p}\sum_{k=1}^{\infty} \frac{1}{k} \frac{\delta_{1}(p^{k})}{p^{ks}} \right)\geq1
$$
因为指数上的每项都 $\displaystyle \geq 0$.
#### Hyperbolic sums
If $\displaystyle F$ is a function defined on pairs of positive integers, there are three ways to calculate 
$$
S_{N}=\sum \sum F(m,n)
$$
where the sum is taken over all pairs of positive integers $\displaystyle (m,n)$ which satisfy $\displaystyle mn\leq N$.
We may carry out the summation in any one of the following three ways:
1. Along hyperbolas:

$$
S_{N}=\sum_{1\leq k\leq N}\left( \sum_{nm=k}F(m,n) \right)
$$
2. Vertically:

$$
S_{N}=\sum_{1\leq m\leq N}\left( \sum_{1\leq n\leq N/m} F(m,n) \right)
$$
3. Horizontally:

$$
S_{N}=\sum_{1\leq n\leq N}\left( \sum_{1\leq m\leq N/n} F(m,n) \right)
$$
![[Stein-I-Fourier Analysis.pdf#page=287&rect=32,421,375,578|Stein-I-Fourier Analysis, p.270]]

#### Intermezzo: the divisor problem
> [!NOTE]
> The divisor is crazy!


For a positive integer $\displaystyle k$, let $\displaystyle d(k)$ denote the number of positive divisors of $\displaystyle k$.
One may notice that the behavior of $\displaystyle d(k)$ as $\displaystyle k$ tends to infinity is rather irregular, and in fact, it does not seem possible to approximate $\displaystyle d(k)$ by a simple analytic expression in $\displaystyle k$.
However, it is natural to inquire about the average size of $\displaystyle d(k)$. i.e.
$$
\frac{1}{N}\sum_{k=1}^{N} d(k)\ \ \ \ \text{as }N\to \infty
$$
> [!IMPORTANT]
> The answer was provided by Dirichlet, who made use of hyperbolic sums.

Indeed, we observe that
$$
d(k)=\sum_{nm=k,\ 1\leq n,m}1
$$
> [!thm]
> If $\displaystyle k$ is a positive integer, then
> $$
\frac{1}{N}\sum_{k=1}^{N}d(k)=\log N+O（1）
$$

More precisely,
$$
\frac{1}{N}\sum_{k=1}^{N}d(k)=\log N+(2\gamma-1)+O(1/N^{1/2})
$$
Proof:
$$
\begin{align}
\sum_{k=1}^{N} d(k) & =\sum_{k=1}^{N} \sum_{nm=k,\ 1\leq n,m}1 \\
 & =\sum_{1\leq m\leq N}\sum_{1\leq n\leq N/m}1 \\
 & =\sum_{1\leq m\leq N}(N/m+O(1)) \\
 & =N\left( \sum_{1\leq m\leq N}1/m \right)+O(N)
\end{align}
$$
于是
$$
\frac{1}{N}\sum_{k=1}^{N} d(k)=\log N+O(1)
$$
The more precise approximation see [[Stein-I-Fourier Analysis.pdf#page=288|Stein-I-Fourier Analysis, p.271]]
See more in stein-I.

